Test cmi on some higher-order impl combinator

src/lowparse/LowParse.SLow.Array.fst
@@ -1,23 +1,8 @@
 module LowParse.SLow.Array
-include LowParse.SLow.FLData
-include LowParse.SLow.VLData
-include LowParse.SLow.List
-include LowParse.Spec.Array
 
 module U32 = FStar.UInt32
 
-inline_for_extraction
-let parse32_array
-  (#k: parser_kind)
-  (#t: Type0)
-  (#p: parser k t)
-  (s: serializer p)
-  (p32: parser32 p)
-  (array_byte_size: nat)
-  (array_byte_size32: U32.t { U32.v array_byte_size32 == array_byte_size } )
-  (elem_count: nat)
-  (u : unit { fldata_array_precond p array_byte_size elem_count == true } )
-: Tot (parser32 (parse_array s array_byte_size elem_count))
+let parse32_array #k #t #p s p32 array_byte_size array_byte_size32 elem_count u
 = [@inline_let]
   let _ =
     fldata_to_array_inj s array_byte_size elem_count u
@@ -34,17 +19,7 @@ let parse32_array
     )
     ()
 
-inline_for_extraction
-let serialize32_array
-  (#k: parser_kind)
-  (#t: Type0)
-  (#p: parser k t)
-  (#s: serializer p)
-  (s32: partial_serializer32 s)
-  (array_byte_size: nat { array_byte_size < 4294967296 } )
-  (elem_count: nat)
-  (u : unit { fldata_array_precond p array_byte_size elem_count == true } )
-: Tot (serializer32 (serialize_array s array_byte_size elem_count u))
+let serialize32_array #k #t #p #s s32 array_byte_size elem_count u
 = [@inline_let]
   let _ =
     fldata_to_array_inj s array_byte_size elem_count u
@@ -65,37 +40,11 @@ let serialize32_array
     (fun x -> array_to_fldata s array_byte_size elem_count u x)
     ()
 
-inline_for_extraction
-let size32_array
-  (#k: parser_kind)
-  (#t: Type0)
-  (#p: parser k t)
-  (s: serializer p)
-  (array_byte_size: nat)
-  (array_byte_size32: U32.t { U32.v array_byte_size32 == array_byte_size } )
-  (elem_count: nat)
-  (u : unit { fldata_array_precond p array_byte_size elem_count == true } )
-: Tot (size32 (serialize_array s array_byte_size elem_count u))
+let size32_array #k #t #p s array_byte_size array_byte_size32 elem_count u
 = size32_constant (serialize_array s array_byte_size elem_count u) array_byte_size32 ()
 
 
-inline_for_extraction
-let parse32_vlarray
-  (array_byte_size_min: nat)
-  (array_byte_size_min32: U32.t { U32.v array_byte_size_min32 == array_byte_size_min } )
-  (array_byte_size_max: nat)
-  (array_byte_size_max32: U32.t { U32.v array_byte_size_max32 == array_byte_size_max } )
-  (#k: parser_kind)
-  (#t: Type0)
-  (#p: parser k t)
-  (s: serializer p)
-  (p32: parser32 p)
-  (elem_count_min: nat)
-  (elem_count_max: nat)
-  (u: unit {
-    vldata_vlarray_precond array_byte_size_min array_byte_size_max p elem_count_min elem_count_max == true  
-  })
-: Tot (parser32 (parse_vlarray array_byte_size_min array_byte_size_max s elem_count_min elem_count_max u))
+let parse32_vlarray array_byte_size_min array_byte_size_min32 array_byte_size_max array_byte_size_max32 #k #t #p s p32 elem_count_min elem_count_max u
 = [@inline_let]
   let _ =
     vldata_to_vlarray_inj array_byte_size_min array_byte_size_max s elem_count_min elem_count_max u
@@ -114,21 +63,7 @@ let parse32_vlarray
     )
     ()
 
-inline_for_extraction
-let serialize32_vlarray
-  (array_byte_size_min: nat)
-  (array_byte_size_max: nat { array_byte_size_max < 4294967292 } ) // NOTE here: max must be less than 2^32 - 4 to account for the size of the length header
-  (#k: parser_kind)
-  (#t: Type0)
-  (#p: parser k t)
-  (#s: serializer p)
-  (s32: partial_serializer32 s)
-  (elem_count_min: nat)
-  (elem_count_max: nat)
-  (u: unit {
-    vldata_vlarray_precond array_byte_size_min array_byte_size_max p elem_count_min elem_count_max == true  
-  })
-: Tot (serializer32 (serialize_vlarray array_byte_size_min array_byte_size_max s elem_count_min elem_count_max u))
+let serialize32_vlarray array_byte_size_min array_byte_size_max #k #t #p #s s32 elem_count_min elem_count_max u
 = [@inline_let]
   let _ =
     vldata_to_vlarray_inj array_byte_size_min array_byte_size_max s elem_count_min elem_count_max u
@@ -150,22 +85,7 @@ let serialize32_vlarray
     (fun x -> vlarray_to_vldata array_byte_size_min array_byte_size_max s elem_count_min elem_count_max u x)
     ()
 
-inline_for_extraction
-let size32_vlarray
-  (array_byte_size_min: nat)
-  (array_byte_size_max: nat { array_byte_size_max < 4294967292 } ) // NOTE here: max must be less than 2^32 - 4 to account for the size of the length header
-  (#k: parser_kind)
-  (#t: Type0)
-  (#p: parser k t)
-  (s: serializer p)
-  (elem_count_min: nat)
-  (elem_count_max: nat)
-  (u: unit {
-    vldata_vlarray_precond array_byte_size_min array_byte_size_max p elem_count_min elem_count_max == true  
-  })
-  (size_header_byte_size32: U32.t { U32.v size_header_byte_size32 == log256' array_byte_size_max } )
-  (elem_byte_size32: U32.t { U32.v elem_byte_size32 == k.parser_kind_low } )
-: Tot (size32 (serialize_vlarray array_byte_size_min array_byte_size_max s elem_count_min elem_count_max u))
+let size32_vlarray array_byte_size_min array_byte_size_max #k #t #p s elem_count_min elem_count_max u size_header_byte_size32 elem_byte_size32
 = [@inline_let]
   let _ =
     vldata_to_vlarray_inj array_byte_size_min array_byte_size_max s elem_count_min elem_count_max u
